theories/trace.v
@@ -7,7 +7,7 @@ Require Import util.
 
 Inductive prov_type: Set :=
   | prov_trans_unary: un_op → prov_type
-  | prov_trans_binary: bin_op → prov_type
+  | prov_trans_binary: ∀ bt, bin_op → type_to_coq_type bt → prov_type
   | prov_agg: agg_op → prov_type
   (* Just re-use it; should be fine. *)
   | prov_udf: trans_op → prov_type
@@ -15,16 +15,30 @@ Inductive prov_type: Set :=
   | prov_join: prov_type
 .
 
-Definition prov_type_eqb τ1 τ2: bool :=
-  match τ1, τ2 with
+Definition prov_type_eqb (τ1 τ2: prov_type): bool.
+  refine (match τ1, τ2 with
   | prov_trans_unary op1, prov_trans_unary op2 => un_op_eqb op1 op2
-  | prov_trans_binary op1, prov_trans_binary op2 => bin_op_eqb op1 op2
+  | prov_trans_binary bt1 op1 v1, prov_trans_binary bt2 op2 v2 => andb (bin_op_eqb op1 op2) _
   | prov_agg op1, prov_agg op2 => agg_op_eqb op1 op2
   | prov_noise op1, prov_noise op2 => noise_op_eqb op1 op2
   | prov_join, prov_join => true
   | prov_udf op1, prov_udf op2 => trans_op_eqb op1 op2
   | _, _ => false
-  end.
+  end).
+  destruct (type_matches bt1 bt2) eqn: Heq.
+  - apply type_matches_eq in Heq. subst.
+    destruct bt2; simpl in *.
+    + destruct (Nat.eqb v1 v2).
+      * apply true.
+      * apply false.
+    + destruct (Bool.eqb v1 v2).
+      * apply true.
+      * apply false.
+    + destruct (String.eqb v1 v2).
+      * apply true.
+      * apply false.
+  - apply false.
+Defined.
 
 Inductive trace_ty: Type :=
   (* ⊥ *)
@@ -33,6 +47,8 @@ Inductive trace_ty: Type :=
   | TrLinear: prov_type → Policy.policy → trace_ty → trace_ty
   (* Branching trace. *)
   | TrBranch: prov_type → Policy.policy → list trace_ty → trace_ty
+  (* Binary expressions *)
+  | TrBinary: prov_type → Policy.policy → trace_ty → trace_ty → trace_ty  
 .
 
 Definition extract_policy tr :=
@@ -40,6 +56,7 @@ Definition extract_policy tr :=
   | TrEmpty p => p
   | TrLinear _ p _ => p
   | TrBranch _ p _ => p
+  | TrBinary _ p _ _ => p
   end.
 
 (*
